\documentclass{article}
\title{Quiz 2}
\author{Tyler Lukasiewicz}


\usepackage{amsmath}

\begin{document}
\maketitle

Prove 
\begin{equation}
    v = \frac{1}{n-1} \sum_{i =1}^n (x_i - \mu)^2 = \frac{1}{n-1} (\sum_{i = 1}^n x_i ^2 -n \mu ^2)
\end{equation}

Solution:

\begin{align*}
    v &= \frac{1}{n-1} \sum_{i =1}^n (x_i - \mu)^2 \\
    &= \frac{1}{n-1}(\sum_{i=1}^n (x_i^2 - 2 x_i \mu  + \mu ^2)) \\
    &= \frac{1}{n-1} (\sum_{i=1}^n x_i^2 - 2 \mu \sum_{i=1}^n x_i + n \mu^2) \\
    &=  \frac{1}{n-1} (\sum_{i=1}^n x_i^2  - 2 n \mu ^2 + n \mu ^2) \\
    &= \frac{1}{n-1}(\sum_{i=1}^n x_2^2 - n \mu ^2)
\end{align*}

\begin{align*}
    error(va): &0.000000000010231815394945442677 \\
    error(vairiance): &0.000000000000000000000000000000
\end{align*}


The better approximation is
\begin{equation*}
     v = \frac{1}{n-1} \sum_{i =1}^n (x_i - \mu)^2 
\end{equation*}

\end{document}
